\documentclass[oneside]{article}

\usepackage{amsfonts}
\usepackage{amsmath}
\usepackage{amssymb}
\usepackage{amsthm}
\usepackage{enumitem}
\usepackage{mathtools}

\allowdisplaybreaks

% Notation shortcuts
\newcommand\abs[1]{\left|#1\right|}
\newcommand\defeq{\overset{\mathrm{def}}{=}}
\newcommand*\Laplace{\mathop{}\!\mathbin\bigtriangleup}

\DeclareMathOperator{\sgn}{sgn}
\DeclareMathOperator{\atantwo}{atan2}

\newcommand\bbC{\mathbb{C}}
\newcommand\bbR{\mathbb{R}}
\newcommand\bbZ{\mathbb{Z}}

\newtheorem*{lem}{Lemma}

\begin{document}
Define $\tau = 2\pi$.

Changing variables $u = x - \tau$, we have\begin{equation}
  \label{eq:first}
  \int_{a+\tau}^{b+\tau}f(x)dx
  = \int_{a}^{b}f(u + \tau)du \\
  = \int_{a}^{b}f(u)du\text,
\end{equation} where in the last equality we use the fact that $f$ is
$\tau$-periodic.

Setting $a = a' - \tau, b = b' - \tau$ in \eqref{eq:first}, we obtain\[
  \int_{a'}^{b'}f(x)dx = \int_{a' - \tau}^{b - \tau}f(x)dx \text{.}
\]

Hence, \[
  \int_{a}^{b}f(x)dx
  = \int_{a + \tau}^{b + \tau}f(x)dx
  = \int_{a - \tau}^{b - \tau}f(x)dx \text{.}
\]

Similarly, we have \begin{align}
  \int_{a}^{\tau + a} f(x) dx
  &= \int_{a}^{\tau} f(x) dx + \int_{\tau}^{\tau + a} f(x) dx
  & \text{(F.T.C.)} \nonumber \\
  &= \int_{a}^{\tau} f(x) dx + \int_{\tau}^{\tau + a} f(x - \tau) dx
  & \text{(periodicity)} \nonumber \\
  &= \int_{a}^{\tau} f(x) dx + \int_{0}^{a} f(u) du
  & \text{($u = x - \tau$)} \nonumber \\
  &= \int_{0}^{\tau} f(x) dx \text{.} \label{eq:second}
\end{align}

Also, \[
  \int_{0}^{\tau}f(x + a)dx = \int_{a}^{\tau + a}f(u)du = \int_0^\tau f(x)dx
\] where the second inequality is by \eqref{eq:second}.

Offsetting $a$ by $\tau/2$, we also obtain\[
  \int_{-\tau/2}^{\tau/2}f(x+a)dx = \int_{-\tau/2}^{\tau/2}f(x)dx
  = \int_{-\tau/2+a}^{\tau/2+a}f(x)dx
\] as desired.

\end{document}
