\documentclass[oneside]{article}

\usepackage{amsfonts}
\usepackage{amsmath}
\usepackage{amssymb}
\usepackage{amsthm}
\usepackage{enumitem}
\usepackage{mathtools}

\allowdisplaybreaks

% Notation shortcuts
\newcommand\abs[1]{\left|#1\right|}
\newcommand\defeq{\overset{\mathrm{def}}{=}}
\newcommand*\Laplace{\mathop{}\!\mathbin\bigtriangleup}

\DeclareMathOperator{\sgn}{sgn}
\DeclareMathOperator{\atantwo}{atan2}

\newcommand\bbC{\mathbb{C}}
\newcommand\bbR{\mathbb{R}}
\newcommand\bbZ{\mathbb{Z}}

\newtheorem*{lem}{Lemma}

\begin{document}
Define $\tau = 2\pi$.
\begin{enumerate}[label=(\alph*)]
  \item We know that \[
      f(\theta) \sim \sum_{n=-\infty}^\infty \hat f(n) e^{in\theta}
    \] Pick $N > 0$ and take the partial sum \[
      S_N(f)(\theta) = \sum_{n=-N}^N\hat f(n)e^{in\theta} \text{.}
    \] Then\begin{align*}
      S_N(f)(\theta)
      &= \hat f(0) + \sum_{0 < \abs{n} \leq N}\hat f(n)e^{in\theta} \\
      &= \hat f(0)
       + \sum_{0 < n \leq N}\hat f(n)e^{in\theta} + \hat f(-n)e^{-in\theta} \\
      &= \hat f(0)
       + \sum_{0 < n \leq N}\hat f(n)[\cos n\theta + i \sin n\theta]
       + \hat f(-n)[\cos -n\theta + i \sin -n\theta] \\
      &= \hat f(0)
       + \sum_{0 < n \leq N}\hat f(n)[\cos n\theta + i \sin n\theta]
       + \hat f(-n)[\cos n\theta - i \sin n\theta] \\
      &= \hat f(0)
       + \sum_{0 < n \leq N} [\hat f(n) + \hat f(-n)]\cos n\theta
         + i[\hat f(n) - \hat f(-n)] \sin n\theta \text{.}
    \end{align*}

    Limiting $N \to \infty$, we obtain\[
      f(\theta) \sim \hat f(0)
       + \sum_{n > 0} [\hat f(n) + \hat f(-n)]\cos n\theta
         + i[\hat f(n) - \hat f(-n)] \sin n\theta\text{.}
    \]\qed

  \item Assume that $f$ is even. Then\begin{align*}
      &\tau\hat f(n) - \tau\hat f(-n) \\
      &= \int_{-\tau/2}^{\tau/2} f(\theta)e^{-in\theta}d\theta
      - \int_{-\tau/2}^{\tau/2} f(\theta)e^{in\theta}d\theta \\
      &= \int_{-\tau/2}^{\tau/2} f(\theta)e^{-in\theta}d\theta
      - \int_{-\tau/2}^{\tau/2} f(-\theta)e^{-in\theta}d\theta
      & \text{(subst. $\theta \coloneqq -\theta$)}\\
      &= \int_{-\tau/2}^{\tau/2} \left[f(\theta) - f(-\theta)\right]e^{-in\theta}d\theta \\
      &= 0\text. &\text{($f(\theta) = f(-\theta)$)}
    \end{align*}

    Hence $\hat f(n) = \hat f(-n)$ and by (a), \[
      f(\theta) \sim \hat f(0)
       + 2\sum_{n > 0} \hat f(n) \cos n\theta\text{.}
    \] \qed

  \item Assume that $f$ is odd. Then\begin{align*}
      &\tau\hat f(n) + \tau\hat f(-n) \\
      &= \int_{-\tau/2}^{\tau/2} f(\theta)e^{-in\theta}d\theta
      + \int_{-\tau/2}^{\tau/2} f(\theta)e^{in\theta}d\theta \\
      &= \int_{-\tau/2}^{\tau/2} f(\theta)e^{-in\theta}d\theta
      + \int_{-\tau/2}^{\tau/2} f(-\theta)e^{-in\theta}d\theta
      & \text{(subst. $\theta \coloneqq -\theta$)}\\
      &= \int_{-\tau/2}^{\tau/2} \left[f(\theta) + f(-\theta)\right]e^{-in\theta}d\theta \\
      &= 0\text. &\text{($f(\theta) = -f(-\theta)$)}
    \end{align*}

    Hence $\hat f(n) = -\hat f(-n)$ and by (a), \[
      f(\theta) \sim \hat f(0)
       + 2i\sum_{n > 0} \hat f(n)\sin n\theta\text{.}
    \] \qed

  \item Suppose that for all $\theta \in \bbR$,
  $f(\theta + \tau/2) = f(\theta)$. Let $n$ be odd. Then \begin{align*}
    \hat f(n)
    &= \int_{-\tau/2}^{\tau/2} f(\theta)e^{-in\theta}d\theta \\
    &= \int_{-\tau/2}^0 f(\theta)e^{-in\theta}d\theta
    + \int_0^{\tau/2} f(\theta)e^{-in\theta}d\theta \\
    &= \int_0^{\tau/2} f(\theta - \tau/2)e^{-in\theta - in\tau/2}d\theta
    + \int_0^{\tau/2} f(\theta)e^{-in\theta}d\theta
    & \text{(subst. $\theta \coloneqq \theta + \tau/2$)} \\
    &= \int_0^{\tau/2} f(\theta)e^{-in\theta}e^{-in\tau/2}d\theta
    + \int_0^{\tau/2} f(\theta)e^{-in\theta}d\theta \\
    &= -\int_0^{\tau/2} f(\theta)e^{-in\theta}d\theta
    + \int_0^{\tau/2} f(\theta)e^{-in\theta}d\theta
    &\text{($e^{in\tau/2} = -1$ for odd $n$)} \\
    &= 0 \text{.}
  \end{align*} \qed

  \item \begin{itemize}[leftmargin=34pt]
    \item[($\implies$)] Let $f$ be real-valued. Then
    for all $\theta$, $\overline{f(\theta)} = f(\theta)$ and \begin{align*}
      \overline{\hat{f}(n)}
      &= \overline{\int_{-\tau/2}^{\tau/2} f(\theta)e^{-in\theta}d\theta} \\
      &= \int_{-\tau/2}^{\tau/2} \overline{f(\theta)e^{-in\theta}}d\theta \\
      &= \int_{-\tau/2}^{\tau/2} \overline{f(\theta)}e^{in\theta}d\theta \\
      &= \int_{-\tau/2}^{\tau/2} f(\theta)e^{in\theta}d\theta \\
      &= \hat{f}(-n)\text{.}
    \end{align*}

    \item[($\impliedby$)] Let $f$ be such that
    $\overline{\hat{f}(n)} = \hat{f}(-n)$ for all $n$. Then \begin{align*}
      \overline{f(\theta)}
      &\sim \overline{\sum_{-\infty}^\infty \hat f(n)e^{in\theta}} \\
      &= \sum_{-\infty}^\infty \overline{\hat f(n)e^{in\theta}} \\
      &= \sum_{-\infty}^\infty \hat f(-n)e^{-in\theta} \\
      &= \sum_{-\infty}^\infty \hat f(n)e^{in\theta} \\
      &\sim f(\theta) \text{.}
    \end{align*} Hence,\[
      \overline f = f
    \] almost everywhere.\qed
  \end{itemize}
\end{enumerate}

\end{document}
