\documentclass[oneside]{article}

\usepackage{amsfonts}
\usepackage{amsmath}
\usepackage{amssymb}
\usepackage{amsthm}
\usepackage{enumitem}
\usepackage{mathtools}

\allowdisplaybreaks

% Notation shortcuts
\newcommand\abs[1]{\left|#1\right|}
\newcommand\defeq{\overset{\mathrm{def}}{=}}
\newcommand*\Laplace{\mathop{}\!\mathbin\bigtriangleup}

\DeclareMathOperator{\sgn}{sgn}
\DeclareMathOperator{\atantwo}{atan2}

\newcommand\bbC{\mathbb{C}}
\newcommand\bbR{\mathbb{R}}
\newcommand\bbZ{\mathbb{Z}}

\newtheorem*{lem}{Lemma}

\begin{document}
  \begin{enumerate}[label=(\alph*)]
    \item
      Observe that \begin{align*}
        \sum_{n=M}^{N-1} (a_{n+1} - a_n)B_n
        &= \sum_{n=M}^{N-1} a_{n+1}B_n - \sum_{n=M}^{N-1} a_nB_n \\
        &= \sum_{n=M+1}^{N} a_{n}B_{n-1} - \sum_{n=M}^{N-1} a_nB_n \\
        &= a_NB_{N-1} - a_MB_M + \sum_{n=M+1}^{N-1} a_{n}(B_{n-1} - B_n) \\
        &= a_NB_{N-1} - a_MB_M - \sum_{n=M+1}^{N-1} a_nb_n \text{.}
      \end{align*}

      Then \begin{align*}
        &a_NB_N - a_MB_{M-1} - \sum_{n=M}^{N-1}(a_{n+1}-a_n)B_n \\
        &= a_NB_N - a_MB_{M-1} - a_NB_{N-1} + a_MB_M
        + \sum_{n=M+1}^{N-1} a_nb_n \\
        &= a_Nb_N + a_Mb_M + \sum_{n=M+1}^{N-1} a_nb_n \\
        &= \sum_{n=M}^{N} a_nb_n \text{.}
      \end{align*}\qed

    \item
      We know that \[
        \sum_{n=1}^N a_nb_n = a_NB_N - \sum_{n=1}^{N-1}(a_{n+1}-a_n)B_n
      \] for all $N = 1, 2, \dots$.

      We are given that $B_N$ is bounded. Let $C > 0$ be such that
      $\abs{B_n} < C$ for all $n = 0, 1, 2, \dots$. Pick an arbitrary
      $\epsilon > 0$. Let $M$ be such that $a_M < \epsilon/2C$. Then for all
      $N > N' > M$, \begin{align*}
        &\abs{\sum_{n=1}^{N} a_nb_n - \sum_{n=1}^{N'} a_nb_n} \\
        &= \abs{a_{N}B_{N} - a_{N'}B_{N'} - \sum_{n=1}^{N-1}(a_{n+1}-a_n)B_n
        + \sum_{n=1}^{N'-1}(a_{n+1}-a_n)B_n} \\
        &= \abs{a_{N}B_{N} - a_{N'}B_{N'} - \sum_{n=N'}^{N-1}(a_{n+1}-a_n)B_n} \\
        &\leq \abs{a_{N}B_{N}} + \abs{a_{N'}B_{N'}}
        + \sum_{n=N'}^{N-1}\abs{(a_{n+1}-a_n)B_n} \\
        &\leq \abs{a_{N}}C + \abs{a_{N'}}C
        + \sum_{n=N'}^{N-1}\abs{a_{n+1}-a_n}C \\
        &= a_{N}C + a_{N'}C + \sum_{n=N'}^{N-1}(a_n - a_{n+1})C
        \qquad\text{($a_n \geq a_{n+1} \geq 0 \;\forall n$)}\\
        &= 2a_{N'}C \\
        &\leq 2a_MC \\
        &< \epsilon\text{.}
      \end{align*} \qed

  \end{enumerate}
\end{document}
