\documentclass[oneside]{article}

\usepackage{amsfonts}
\usepackage{amsmath}
\usepackage{amssymb}
\usepackage{amsthm}
\usepackage{enumitem}
\usepackage{mathtools}

\allowdisplaybreaks

% Notation shortcuts
\newcommand\abs[1]{\left|#1\right|}
\newcommand\defeq{\overset{\mathrm{def}}{=}}
\newcommand*\Laplace{\mathop{}\!\mathbin\bigtriangleup}

\DeclareMathOperator{\sgn}{sgn}
\DeclareMathOperator{\atantwo}{atan2}

\newcommand\bbC{\mathbb{C}}
\newcommand\bbR{\mathbb{R}}
\newcommand\bbZ{\mathbb{Z}}

\newtheorem*{lem}{Lemma}

\begin{document}
Let $f : [-\pi, \pi] \to \bbR$ such that \[
  f(\theta) = \begin{cases}
    0 & \text{if }\abs{\theta} > \delta \text{,} \\
    1 - \abs{\theta}/\delta & \text{if }\abs{\theta} \leq \delta \text{.}
  \end{cases}
\]

$f$ is even, so its Fourier series is cosine with coefficients\[
  A_n = \frac{1}{2\pi}\int_{-\pi}^\pi f(\theta)\cos n\theta d\theta \text{.}
\]

For $n = 0$, we have \begin{align*}
  A_0
  &= \frac{1}{2\pi}\int_{-\pi}^\pi f(\theta) d\theta \\
  &= \frac{1}{2\pi}\int_{-\delta}^\delta
  \left(1 - \frac{\abs{\theta}}{\delta}\right) d\theta \\
  &= \frac{1}{\pi}\int_0^\delta
  \left(1 - \frac{\theta}{\delta}\right) d\theta \\
  &= \frac{\delta}{2\pi} \text{.}
\end{align*} For $n = 1, 2, \dots$, we have\begin{align*}
  A_{n} = A_{-n} &= \frac{1}{\pi}\int_0^\delta
  \left(1 - \frac{\theta}{\delta}\right) \cos n\theta d\theta \\
  &= \frac{1}{\pi}\int_0^\delta \cos n\theta d\theta
   - \frac{1}{\pi\delta}\int_0^\delta \theta \cos n\theta d\theta \\
  &= \frac{\sin n\delta}{\pi n}
   - \frac{n\delta\sin n\delta + \cos n\delta - 1}{n^2\pi\delta} \\
  &= \frac{1 - \cos n\delta}{n^2\pi\delta}
\end{align*}

Hence, \[
  f(\theta)
  \sim \frac{\delta}{2\pi}
  + 2\sum_{n=1}^\infty \frac{1 - \cos n\delta}{n^2\pi\delta}\cos n\theta
  \text{.}
\] We conclude by proving equality. It is easy to see that $f$ is a continuous
function on the circle. We can bound \[
  \abs{\frac{1 - \cos n\delta}{n^2 \pi \delta}} \leq \frac{2}{n^2\pi\delta}
  \text{,}
\] so $\sum_{n=1}^\infty A_n$ is absolutely convergent. Hence, by corollary 2.3,
\[
  f(\theta)
  = \frac{\delta}{2\pi}
  + 2\sum_{n=1}^\infty \frac{1 - \cos n\delta}{n^2\pi\delta}\cos n\theta
  \text{.}
\]\qed
\end{document}
