\documentclass[oneside]{article}

\usepackage{amsfonts}
\usepackage{amsmath}
\usepackage{amssymb}
\usepackage{amsthm}
\usepackage{enumitem}
\usepackage{mathtools}
\usepackage{cleveref}

\allowdisplaybreaks

% Notation shortcuts
\newcommand\abs[1]{\left|#1\right|}
\newcommand\norm[1]{\left\|#1\right\|}
\newcommand\defeq{\overset{\mathrm{def}}{=}}
\newcommand*\Laplace{\mathop{}\!\mathbin\bigtriangleup}

\DeclarePairedDelimiter\ceil{\lceil}{\rceil}
\DeclarePairedDelimiter\floor{\lfloor}{\rfloor}

\DeclareMathOperator{\sgn}{sgn}
\DeclareMathOperator{\atantwo}{atan2}

\newcommand\bbC{\mathbb{C}}
\newcommand\bbR{\mathbb{R}}
\newcommand\bbQ{\mathbb{Q}}
\newcommand\bbZ{\mathbb{Z}}

\newtheorem*{lem}{Lemma}
\newtheorem*{cor}{Corollary}

\renewcommand{\thefootnote}{[\arabic{footnote}]}

\begin{document}
  \begin{proof}
    Consider the sequence $\{A_n\}_{n=1}^\infty$ where $A_n = \{a_{n,k}\}_{k\in\bbZ}$.

    For every $k \in \bbZ$, the sequence $\{a_{n,k}\}_{n=1}^\infty$ is Cauchy since $\abs{a_{n,k} - a_{m,k}}$ is bounded by $\norm{A_n - A_m}$ for all $n, m \in \{1, 2, \dots \}$. By completeness of $\bbC$\footnote{See exercise 1.} $\{a_{n,k}\}_{n=1}^\infty$ converges to some $b_k$.

    Let $B = (\dots, b_{-1}, b_0, b_1, \dots)$. Since $\{A_n\}_{n=1}^\infty$ is Cauchy, for all $\epsilon>0$ there exists $N$ such that for all $n, m > N$, \[
      \sum_{k=-K}^K \abs{a_{n,k} - a_{m,k}}^2
      \leq \norm{A_n - A_m}^2 < \epsilon \text{.}
    \] Limiting $m \to \infty$, we obtain \[
      \sum_{k=-K}^K \abs{a_{n,k} - b_k}^2
      \leq \epsilon \text{.}
    \] By the monotonic convergence theorem, we can limit $K \to \infty$ and obtain\[
      \abs{A_n - B}^2 \leq \epsilon \text{,}
    \] so $\abs{A_n - B} \to 0$ as $n \to \infty$.

    Finally, we must prove that $B \in \ell^2(\bbZ)$. Pick $n$ such that $\norm{A_n - B} < 1$. Then $A_n - B \in \ell^2(\bbZ)$, so $B = A_n - (A_n - B) \in \ell^2(\bbZ)$ since vector spaces are closed under addition.
  \end{proof}
\end{document}
