\documentclass[oneside]{article}

\usepackage{amsfonts}
\usepackage{amsmath}
\usepackage{amssymb}
\usepackage{amsthm}
\usepackage{enumitem}
\usepackage{mathtools}
\usepackage{pgfplots}

\allowdisplaybreaks

% Notation shortcuts
\newcommand\abs[1]{\left|#1\right|}
\newcommand\defeq{\overset{\mathrm{def}}{=}}
\newcommand*\Laplace{\mathop{}\!\mathbin\bigtriangleup}

\DeclareMathOperator{\sgn}{sgn}
\DeclareMathOperator{\atantwo}{atan2}

\newcommand\bbC{\mathbb{C}}
\newcommand\bbR{\mathbb{R}}
\newcommand\bbZ{\mathbb{Z}}

\newtheorem*{lem}{Lemma}

\begin{document}
  \begin{enumerate}[label=(\alph*)]
    \item\hspace{0pt}

      \begin{tikzpicture}[
        declare function={
          func(\x)= (\x<0) * -x + (\x >= 0) * x;
        }
      ]
      \begin{axis}[
       width=.88\textwidth,
       height=.6\textwidth,
        axis x line=middle, axis y line=middle,
        ymin=-0, ymax=3.5, ytick={0,...,3}, ylabel=$f(\theta)$,
        xmin=-pi, xmax=pi, xtick={
          -3.14159, -1.5708, 1.5708, 3.14159
      },
      xticklabels={
          $-\pi$, $-\frac{\pi}{2}$, $\frac{\pi}{2}$, $\pi$
      },
      xlabel=$\theta$,
      ]
      \addplot[black, domain=-pi:pi, smooth]{func(x)};
      \end{axis}
      \end{tikzpicture}

    \item The Fourier coefficients are\begin{align*}
      \hat f(n)
      &= \frac{1}{2\pi}\int_{-\pi}^\pi \abs{\theta} e^{-in\theta} d\theta \\
      &= \frac{1}{2\pi}\int_{-\pi}^\pi \abs{\theta} \cos n\theta d\theta
      - \frac{1}{2\pi}i\int_{-\pi}^\pi \abs{\theta} \sin n\theta d\theta
      \text{.}
    \end{align*}

    $\abs{\theta} \cos n\theta$ is even and $\abs{\theta} \sin n\theta$ is odd,
    so \[
      \hat f(n) = \frac{1}{\pi}\int_{0}^\pi \theta \cos n\theta d\theta \text{.}
    \]

    We have $\hat f(0) = \pi/2$. For $n \neq 0$, we have \begin{align*}
      \hat f(n) &= \frac{1}{\pi}\int_{0}^\pi \theta \cos n\theta d\theta \\
      &= \frac{\cos\pi n +\pi n \sin\pi n - 1}{\pi n^2} \\
      &= \frac{-1 + (-1)^n}{\pi n^2}
    \end{align*} \qed

    \item The series is cosine since $f$ is even, so \[
      f(\theta)
      \sim \frac{\pi}{2} +
      \sum_{n\neq0}\frac{-1 + (-1)^n}{\pi n^2}\cos n \theta \text{.}
    \]

    Eliminating zero terms,\begin{equation}
      \label{eq:fourier-series}
      f(\theta)
      \sim \frac{\pi}{2} -
      \frac{4}{\pi}\sum_{n\text{ odd}\geq1}\frac{\cos n \theta}{n^2} \text{.}
    \end{equation}

    \item Observe that $\sum\abs{n^{-2}}$ converges absolutely, so we have
    equality in \eqref{eq:fourier-series}. Taking $\theta = 0$, we get
    \begin{align*}
      &0 = \frac{\pi}{2} -
      \frac{4}{\pi}\sum_{n\text{ odd}\geq1}\frac{1}{n^2} \\
      &\iff \sum_{n\text{ odd}\geq1}\frac{1}{n^2} = \frac{\pi^2}{8} \text{.}
    \end{align*}

    From example 2 in section 1.1, we have \[
      g(\theta)
      \sim \frac{\pi^2}{12} + \sum_{n=1}^\infty \frac{\cos n\theta}{n^2}
    \] when $g(\theta) = (\pi-\theta)^2/4$ for $0 \leq \theta \leq 2\pi$. Since
    $\sum n^{-2}$ converges absolutely, we also have equality. Taking
    $\theta = 0$,\begin{align*}
      &\frac{\pi^2}{4} = \frac{\pi^2}{12}+\sum_{n=1}^\infty \frac{1}{n^2} \\
      &\iff \sum_{n=1}^\infty \frac{1}{n^2} = \frac{\pi^2}{6} \text{.}
    \end{align*}\qed


  \end{enumerate}
\end{document}
