\documentclass[oneside]{article}

\usepackage{amsfonts}
\usepackage{amsmath}
\usepackage{amssymb}
\usepackage{amsthm}
\usepackage{enumitem}
\usepackage{mathtools}

\allowdisplaybreaks

% Notation shortcuts
\newcommand\abs[1]{\left|#1\right|}
\newcommand\defeq{\overset{\mathrm{def}}{=}}

\DeclareMathOperator{\sgn}{sgn}

\newcommand\bbC{\mathbb{C}}
\newcommand\bbR{\mathbb{R}}
\newcommand\bbZ{\mathbb{Z}}

\begin{document}
  Let $f : \bbR \to \bbR$ be twice continuously differentiable such that
  \begin{equation}
    \label{eq:ode}
    f''(t) + c^2f(t) = 0
  \end{equation} with $c \neq 0$.

  Let\begin{align*}
    g(t) &= f(t)\cos ct - c^{-1} f'(t) \sin ct \text{,}\\
    h(t) &= f(t)\sin ct + c^{-1} f'(t) \cos ct \text.
  \end{align*} Observe that they are once differentiable. Differentiating,
  \begin{align*}
    g'(t)
    &= f'(t)\cos ct - cf(t)\sin ct - c^{-1} f''(t) \sin ct - f'(t) \cos ct \\
    &= - cf(t)\sin ct - c^{-1} f''(t) \sin ct \\
    &= - cf(t)\sin ct + c f(t) \sin ct & \text{(by \eqref{eq:ode})}\\
    &= 0 \text{,} \\
    h'(t)
    &= f'(t)\sin ct + cf(t)\cos ct + c^{-1} f''(t) \cos ct - f'(t) \sin ct \\
    &= cf(t)\cos ct + c^{-1} f''(t) \cos ct \\
    &= cf(t)\cos ct - cf(t) \cos ct \\
    &= 0 \text{.}
  \end{align*} Thus $g$ and $h$ are constant. Let $a$ and $b$ be constants such
  that \begin{align*}
    g(t) &= f(t)\cos ct - c^{-1} f'(t) \sin ct = a \text{,} \\
    h(t) &= f(t)\sin ct + c^{-1} f'(t) \cos ct = b \text{.}
  \end{align*}

  Then \[
    c^{-1}f'(t)\sin ct = f(t)\cos ct - a
  \] and \[
    f(t)(\sin ct)^2 + c^{-1} f'(t) \sin ct\cos ct = b\sin ct \text{,}
  \] so \begin{align*}
    &f(t)(\sin ct)^2 + (f(t)\cos ct - a)\cos ct = b\sin ct \\
    &\iff f(t)(\sin ct)^2 + f(t)(\cos ct)^2 = a\cos ct + b\sin ct \\
    &\iff f(t) = a\cos ct + b\sin ct \text{.}
  \end{align*}\qed
\end{document}
