\documentclass[oneside]{article}

\usepackage{amsfonts}
\usepackage{amsmath}
\usepackage{amssymb}
\usepackage{amsthm}
\usepackage{enumitem}
\usepackage{mathtools}

\allowdisplaybreaks

% Notation shortcuts
\newcommand\abs[1]{\left|#1\right|}
\newcommand\defeq{\overset{\mathrm{def}}{=}}

\newcommand\bbR{\mathbb{R}}

\begin{document}
  \begin{enumerate}[label=\textbf{(\alph*)}]
    \item $\abs{z}$ is the distance from $z$ to the origin.

    \item \begin{align*}
      & \abs{z} \defeq \left(x^2 + y^2\right)^{1/2} = 0 \\
      &\iff
        x^2 + y^2 = 0 \\
      &\iff
        x^2 = 0\text{ and }y^2 = 0 &
        \text{($x, y \in \bbR$, so $x^2, y^2 \geq 0$)} \\
      &\iff
        x = 0\text{ and }y = 0 \\
      &\iff
        z \defeq x + iy = 0
    \end{align*} \qed

    \item We have $\lambda z = (\lambda x) + i (\lambda y)$ for some
      $\lambda \in \bbR$. Substituting into the definition of the modulus,
      \begin{align*}
        \abs{\lambda z} =
        &\left((\lambda x)^2 + (\lambda y)^2\right)^{1/2} \\
        = & \left(\lambda^2\right)^{1/2}\left(x^2 + y^2\right)^{1/2} \\
        = & \abs{\lambda}\abs{z} \text{.}
      \end{align*}
      \qed

    \item Let $z_1 \defeq x_1 + iy_1$ and $z_2 \defeq x_2 + iy_2$ for some
      $x_1, x_2, y_1, y_2 \in \bbR$.

      We first show that $\abs{z_1z_2} = \abs{z_1}\abs{z_2}$. We have
      \begin{align*}
        z_1z_2
        & = x_1x_2 + ix_1y_2 + ix_2y_1 + i^2y_1y_2 \\
        & = (x_1x_2 - y_1y_2) + i(x_1y_2 + x_2y_1)\text{.}
      \end{align*}
      Substituting into the definition of the modulus,
      \begin{align*}
        \abs{z_1z_2}^2 &= (x_1x_2 - y_1y_2)^2+(x_1y_2 + x_2y_1)^2 \\
        &= \left(x_1^2x_2^2 - 2x_1x_2y_1y_2 + y_1^2y_2^2\right)
          + \left(x_1^2y_2^2 + 2x_1x_2y_1y_2 + x_2^2y_1^2\right) \\
        &= x_1^2x_2^2 + x_1^2y_2^2 + x_2^2y_1^2 + y_1^2y_2^2 \\
        &= \left(x_1^2 + y_1^2\right)\left(x_2^2 + y_2^2\right) \\
        &= \abs{z_1}^2\abs{z_2}^2 \text{.}
      \end{align*}
      Taking the square root of both sides concludes the proof.

      We now show that $\abs{z_1 + z_2} \leq \abs{z_1} + \abs{z_2}$. We have
      \[
        z_1 + z_2 = (x_1 + x_2) + i(y_1 + y_2) \text.
      \]
      By algebra,
      \begin{align*}
        & 0 \leq (x_1y_2-x_2y_1)^2 \\
        & \iff 0 \leq x_1^2y_2^2 - 2x_1x_2y_1y_2 + x_2^2y_1^2 \\
        & \iff 2x_1x_2y_1y_2 \leq x_1^2y_2^2 + x_2^2y_1^2 \\
        & \iff x_1^2x_2^2 + 2x_1x_2y_1y_2 + y_1^2y_2^2
          \leq x_1^2x_2^2 + x_1^2y_2^2 + x_2^2y_1^2 + y_1^2y_2^2 \\
        & \iff (x_1x_2 + y_1y_2)^2
          \leq \left(x_1^2 + y_1^2\right)\left(x_2^2 + y_2^2\right) \\
        & \implies x_1x_2 + y_1y_2
          \leq \sqrt{x_1^2 + y_1^2}\sqrt{x_2^2 + y_2^2} \hspace{20pt} \text{ (since $\mathrm{RHS} \geq 0$)} \\
        & \iff x_1^2 + 2x_1x_2 + x_2^2 + y_1^2 + 2y_1y_2 + y_2^2
          \\&\hspace{40pt} \leq x_1^2 + y_1^2
            + 2\sqrt{x_1^2 + y_1^2}\sqrt{x_2^2 + y_2^2}
            + x_2^2 + y_2^2 \\
        & \iff (x_1 + x_2)^2 + (y_1 + y_2)^2
          \leq \left(\sqrt{x_1^2 + y_1^2} + \sqrt{x_2^2 + y_2^2}\right)^2 \\
        & \iff \sqrt{(x_1 + x_2)^2 + (y_1 + y_2)^2}
          \leq \sqrt{x_1^2 + y_1^2} + \sqrt{x_2^2 + y_2^2} \\
        & \iff \abs{z_1 + z_2} \leq \abs{z_1} + \abs{z_2} \text{.}
      \end{align*}\qed

    \item Observe that \begin{align*}
        \frac{1}{z} &= \frac{1}{x + iy} \\
        &= \frac{x - iy}{(x + iy)(x - iy)} \\
        &= \frac{x - iy}{x^2 + y^2}\text.
      \end{align*}

      Thus \begin{align*}
        \abs{\frac{1}{z}} &= \abs{\frac{x - iy}{x^2 + y^2}} \\
        &= \frac{1}{x^2 + y^2}\abs{x - iy} & \text{(by (c))}
      \end{align*}

      Observing that the definition of $\abs{z}$ depends only on $x^2$ and
      $y^2$, $\abs{x-iy} = \abs{x + iy} = \abs{z}$. Observe also that
      $\abs{z}^2 = x^2 + y^2$ by squaring both sides of its definition. Then \[
        \abs{\frac{1}{z}} = \frac{1}{\abs{z}^2}\abs{z} = \frac{1}{\abs{z}}.
      \]
      \qed

  \end{enumerate}
\end{document}
